feat(completeness): completeness theorem

src/completeness.lean
@@ -1,28 +1,33 @@
-import language_extension consistency
+import language_extension consistency lindenbaum
 open encodable
 
 universes u
 
 namespace fopl
+
+@[simp] lemma app_concat {α β : Type*} (a : α) (s : ℕ → α) (g : α → β) :
+  (λ x, g ((a ⌢ s) x)) = g a ⌢ g ∘ s :=
+by { funext x, cases x; simp  }
+
+@[simp] lemma app_concat' {α β γ : Type*} (a : α) (s : ℕ → α) (g : α → β) (h : β → γ):
+  (λ x, h (g ((a ⌢ s) x))) = h (g a) ⌢ h ∘ g ∘ s :=
+by { funext x, cases x; simp  }
+
 open term formula
 variables (L : language.{u}) (T : theory L)
 
 namespace henkin
-open language language.extension language.consts_pelimination theory
+open language language.extension language.consts_pelimination theory language.language_translation
 
 @[reducible] def extend : language.{u} := L + consts (formula L)
-
-@[reducible] def Lang : ℕ → language
-| 0     := L
-| (n+1) := extend (Lang n)
-
-def Consts : Type u := Σ n, formula (Lang L n)
 
 variables {L}
 
 def henkin_axiom (p : formula L) : formula (extend L) := (∐ ↑p) ⟶ rew ı[0 ⇝ p] ↑p
 
 @[reducible] def theory_extend : theory (extend L) := ↑T ∪ set.range henkin_axiom
+
+variables {T}
 
 section
 open axiomatic_classical_logic axiomatic_classical_logic' provable
@@ -66,9 +71,9 @@ lemma consts_of_henkin_axiom {p : formula L} {c} (mem : c ∈ consts_of_p (henki
 begin
   simp[henkin_axiom, consts_of_p] at mem,
   rcases mem with ⟨t, (t_mem | t_mem), c_mem⟩,
-  { rcases language_translation_coe.fun_formula_inversion_of_mem t_mem with ⟨t, t_mem, rfl⟩, simp at c_mem, contradiction },
+  { rcases language_translation_coe.fun_p_inversion_of_mem t_mem with ⟨t, t_mem, rfl⟩, simp at c_mem, contradiction },
   { rcases formula.rew_inversion_or_le_of_mem_rew t_mem with (⟨t, t_mem', k, rfl⟩ | ⟨k, n, le⟩),
-    { rcases language_translation_coe.fun_formula_inversion_of_mem t_mem' with ⟨t, t_mem'', rfl⟩,
+    { rcases language_translation_coe.fun_p_inversion_of_mem t_mem' with ⟨t, t_mem'', rfl⟩,
       simp[subst_pow] at c_mem,
       rcases mem_of_consts_of_t_subst _ _ _ c_mem with (c_mem | c_mem),
       { simp at c_mem, contradiction },
@@ -88,7 +93,7 @@ end
 theorem theory_extend_consistent (consis : T.consistent) : (theory_extend T).consistent :=
 begin
   have : (↑T : theory (extend L)).consistent, from language.add_consts.consistent_iff.mpr consis,
-  refine of_finite_induction this _,
+  refine consistent.of_finite_induction this _,
   intros s s_ss φ φ_mem p_nmem s_fin consis',
   let U := ↑T ∪ s,
   rcases φ_mem with ⟨φ, rfl⟩,
@@ -108,6 +113,413 @@ begin
   exact consistent_of_disjoint ([φ]) consis' disj (henkin_axiom φ) (by simp; exact this)
 end
 
+variables (L) (T)
+
+@[reducible] def Lang : ℕ → language
+| 0     := L
+| (n+1) := extend (Lang n)
+
+local notation `L[` n `]` := Lang L n
+
+@[reducible] def Consts : Type u := Σ n, formula (Lang L n)
+
+def pConsts (m : ℕ) : Type u := Σ (n : {n | m ≤ n}), formula (Lang L n)
+
+@[reducible] def limit : language := L + consts (Consts L)  
+
+local notation `Lω` := limit L
+
+local infix ` ≃∘ `:50 := ((≃) : term Lω → term Lω → formula Lω)
+
+@[reducible] def Ln_to_Lω : Π n, L[n] ↝ᴸ Lω
+| 0     := add_left
+| (n+1) := let σ : consts (formula L[n]) ↝ᴸ consts (Consts L) := consts_of_fun (λ p, ⟨n, p⟩) in
+    (Ln_to_Lω n).sum (add_right.comp σ)
+
+def pConsts_to_add_pConsts (n : ℕ) : consts (pConsts L n) ↝ᴸ consts (formula L[n]) + consts (pConsts L (n + 1)) :=
+{ fn := λ m f, by { rcases m,
+    { rcases f with ⟨⟨i, hi⟩, p⟩, simp at hi p,
+      by_cases e : i = n,
+      { rcases e with rfl, refine sum.inl p },
+      { have : n + 1 ≤ i, from nat.succ_le_iff.mpr ((ne.symm e).le_iff_lt.mp hi), refine sum.inr ⟨⟨i, this⟩, p⟩ } },
+    { rcases f } },
+  pr := λ m r, by { rcases r } }
+
+@[reducible] def Lω_to_Ln_add_pConsts : Π n, Lω ↝ᴸ L[n] + consts (pConsts L n)
+| 0       := (1 : L ↝ᴸ L).add (consts_of_fun (λ ⟨n, p⟩, ⟨⟨n, by simp⟩, p⟩))
+| (n + 1) :=
+  let τ : L[n] + consts (pConsts L n) ↝ᴸ L[n + 1] + consts (pConsts L (n + 1)) := (add_assoc'_inv _ _ _).comp ((1 : L[n] ↝ᴸ L[n]).add ( pConsts_to_add_pConsts L n)) in
+    τ.comp (Lω_to_Ln_add_pConsts n)
+
+lemma pConsts_to_add_pConsts_of_eq {n : ℕ} (p : formula L[n]) :
+  (pConsts_to_add_pConsts L n).fn 0 (consts.c ⟨⟨n, by { show n ≤ n, by refl }⟩, p⟩) = sum.inl p :=
+by simp[pConsts_to_add_pConsts, consts.c]
+
+lemma pConsts_to_add_pConsts_of_lt {n m : ℕ} (p : formula L[m]) (lt : n < m) :
+  (pConsts_to_add_pConsts L n).fn 0 (consts.c ⟨⟨m, le_of_lt lt⟩, p⟩) = sum.inr (consts.c ⟨⟨m, nat.succ_le_iff.mpr lt⟩, p⟩) :=
+by simp[pConsts_to_add_pConsts, consts.c, show ¬m = n, from ne_of_gt lt]
+
+lemma Lω_to_Ln_add_pConst_fn_of_le {n m : ℕ} (p : formula L[m]) (le : n ≤ m) :
+  (Lω_to_Ln_add_pConsts L n).fn 0 (show (consts (Consts L)).fn 0, from ⟨m, p⟩) = sum.inr (consts.c ⟨⟨m, le⟩, p⟩) :=
+begin
+  simp,
+  induction n with n IH generalizing p m; simp[Lω_to_Ln_add_pConsts, ← coe_fn₂],
+  { refl },
+  { simp[IH p (nat.le_of_succ_le le), ← coe_fn₂],
+    have : n < m, from nat.succ_le_iff.mp le,
+    simp[pConsts_to_add_pConsts_of_lt L p this, ←coe_fn₂] }
+end
+
+lemma commutative (n : ℕ) : (Lω_to_Ln_add_pConsts L n).comp (Ln_to_Lω L n) = add_left :=
+begin
+  induction n with n IH,
+  { ext; simp[Ln_to_Lω, Lω_to_Ln_add_pConsts, add_left_fn_to_coe, add_left_pr_to_coe] },
+  { ext m,
+    { rcases f; simp[Ln_to_Lω, limit, ←coe_fn₁, ←coe_fn₂],
+      { have : (Lω_to_Ln_add_pConsts L n).fn m ((Ln_to_Lω L n).fn m f) = ↑f,
+        { have := (language_translation.eq_iff.mp IH).1 m f, simpa using this },
+        simp[this, add_left_fn_to_coe] },
+      { rcases m,
+        { simp[add_right_fn_to_coe],
+          have := Lω_to_Ln_add_pConst_fn_of_le L f (by refl), simp at this,
+          simp[this, ←coe_fn₂, ←coe_fn₁, add_left_fn_to_coe, pConsts_to_add_pConsts_of_eq L f,
+            show (pConsts_to_add_pConsts L n).fn 0 (consts.c ⟨⟨n, show n ≤ n, by refl⟩, f⟩) = _, from pConsts_to_add_pConsts_of_eq L f] },
+        { rcases f } } },
+    { intros m r, rcases r; simp[Ln_to_Lω, limit, ←coe_pr₁, ←coe_pr₂], 
+      { have : (Lω_to_Ln_add_pConsts L n).pr m ((Ln_to_Lω L n).pr m r) = ↑r,
+        { have := (language_translation.eq_iff.mp IH).2 m r, simpa using this },
+        simp[this, add_left_pr_to_coe] },
+      { rcases r } } }
+end
+
+lemma add_left_Ln_to_Lω_commutative (n : ℕ) : (Ln_to_Lω L (n + 1)).comp (add_left : L[n] ↝ᴸ L[n+1]) = Ln_to_Lω L n :=
+by ext; simp[Ln_to_Lω, add_left_fn_to_coe, add_left_pr_to_coe]
+
+variables {L}
+
+def Lω_seq_limit : seq_limit (Lang L) Lω :=
+{ seq := λ n, add_left,
+  to_limit := Ln_to_Lω L,
+  commutes := add_left_Ln_to_Lω_commutative L,
+  rank_fn := λ n f, by { rcases f, { exact 0 }, { rcases n, { rcases f with ⟨m, f⟩, exact (m + 1) }, { rcases f } } },
+  rank_pr := λ n r, by { rcases r, { exact 0 }, { rcases r } },
+  fn := λ n f, by { rcases f, { exact f }, { rcases n, { rcases f with ⟨m, f⟩, exact sum.inr (consts.c f) }, { rcases f } } },
+  pr := λ n r, by { rcases r, { exact r }, { rcases r } },
+  fn_spec := λ n f, by { rcases f, { refl }, { cases n, { rcases f with ⟨m, f⟩, refl }, { rcases f } } },
+  pr_spec := λ n r, by { rcases r, { refl }, { rcases r } } }
+
+def retruct (p : formula Lω) : formula L[Lω_seq_limit.rank_p p] := Lω_seq_limit.retruct_p p
+
+def henkin_constant (p : formula (limit L)) : Consts L := ⟨Lω_seq_limit.rank_p p, retruct L p⟩
+
+@[simp] lemma retruct_s_c (p : formula Lω) : (Ln_to_Lω L _).fun_p (retruct L p) = p := Lω_seq_limit.retruct_p_spec p 
+
+@[simp] lemma retruct_s (p : formula Lω) : (Ln_to_Lω L _).fun_p (retruct L p) = p := Lω_seq_limit.retruct_p_spec p 
+
+lemma Ln_to_Lω_fun_p_coe (n : ℕ) (p : formula L[n]) :
+  (Ln_to_Lω L (n + 1)).fun_p (by simp[Lang]; refine p) = (Ln_to_Lω L n).fun_p p :=
+by simp[←add_left_Ln_to_Lω_commutative L n, comp_fun_p]; refl
+
+@[simp] lemma Ln_to_Lω_fun_t_coe {n} (p : formula L[n]) :
+  (Ln_to_Lω L (n + 1)).fun_t (↑(↑p : term (consts (formula L[n]))) : term (extend L[n])) = ↑(⟨n, p⟩ : Consts L) :=
+begin
+  unfold_coes, simp[Ln_to_Lω],
+  suffices : ((Ln_to_Lω L n).sum (add_right.comp (consts_of_fun (sigma.mk n)))).fn 0 (↑(consts.c p)) = ↑(consts.c (⟨n, p⟩ : Consts L)),
+  { exact this },
+  simp, refl
+end
+
+variables (T) {L}
+
+@[reducible] def Thy : Π n : ℕ, theory (Lang L n)
+| 0       := T
+| (n + 1) := theory_extend (Thy n)
+
+def Thy' (n : ℕ) := (Ln_to_Lω L n).fun_theory (Thy T n)
+
+local notation `T[` n `]` := Thy' T n
+
+def theory_limit : theory Lω := ⋃ n, T[n]
+
+local notation `Tω` := theory_limit L T
+
+lemma Thy'_ss (n : ℕ) : T[n] ⊆ T[n + 1] :=
+begin
+  simp[fun_theory, Thy', Thy],
+  intros p mem, simp[Lang], refine ⟨by simp[Lang]; refine p, _⟩,
+  simpa[mem] using Ln_to_Lω_fun_p_coe _ n p,
+end
+
+lemma Tn_consistent (consis : T.consistent) (n : ℕ) : theory.consistent T[n] :=
+begin
+  have : theory.consistent (Thy T n),
+  { induction n with n IH, { exact consis }, { exact theory_extend_consistent IH } },
+  have consis' : theory.consistent (add_left.fun_theory (Thy T n) : theory (L[n] + consts (pConsts L n))), from add_consts.consistent_iff.mpr this,
+  have : (add_left.fun_theory (Thy T n) : theory (L[n] + consts (pConsts L n))) = (Lω_to_Ln_add_pConsts L n).fun_theory T[n],
+  { rw[fun_theory, ←commutative, comp_fun_p, set.image_comp], simp[fun_theory, Thy'] },
+  rw this at consis',
+  exact language.language_translation.consistency _ _ consis'
+end
+
+theorem Tω_consistent (consis : T.consistent) : theory.consistent Tω :=
+(theory.consistent.Union_seq (Thy' T) (Thy'_ss T)).mpr (Tn_consistent T consis)
+
+
+lemma T_ss_Tω : ↑T ⊆ Tω :=
+by simpa [show ↑T = T[0], by refl, theory_limit] using set.subset_Union (Thy' T) 0
+
+lemma henkin_mem_Tω (p : formula Lω) : (∐ p) ⟶ rew ı[0 ⇝ henkin_constant p] p ∈ Tω :=
+begin
+  simp[henkin_constant],
+  let r := Lω_seq_limit.rank_p p,
+  suffices : (∐ p) ⟶ rew ı[0 ⇝ henkin_constant p] p ∈ T[r + 1],
+  { simp[theory_limit], refine ⟨_, this⟩ },
+  have lmm₁ : (∐ p) ⟶ rew ı[0 ⇝ henkin_constant p] p = (Ln_to_Lω L (r + 1)).fun_p (henkin_axiom (retruct L p)),
+  { have := Ln_to_Lω_fun_p_coe L r (retruct L p), simp at this, simp[this, henkin_axiom, henkin_constant] },
+  have lmm₂ : (Ln_to_Lω L (r + 1)).fun_p (henkin_axiom (retruct L p)) ∈ T[r + 1],
+  { simp[Thy'], refine ⟨henkin_axiom (retruct L p), by simp[Thy], rfl⟩ },
+  rw lmm₁, exact lmm₂
+end
+
+local notation `Tω⁺` := consistent.maximal Tω
+
+local notation `Lω` := limit _
+
+open axiomatic_classical_logic axiomatic_classical_logic' provable
+
+def Consts.of (t : term Lω) : Consts L := henkin_constant ((t^1) ≃∘ #0)
+#check Consts.of
+
+def Consts.fn {n} (f : (limit L).fn n) (v : finitary (Consts L) n) : Consts L := Consts.of (app f (λ i, (v i)))
+
+def Consts.pr {n} (r : (limit L).pr n) (v : finitary (Consts L) n) : Prop := formula.app r (λ i, (v i)) ∈ Tω⁺
+
+def Consts.equal (p q : Consts L) : Prop := (p ≃∘ q) ∈ Tω⁺
+
+local notation p ` ~[`:50 T :50 `] `:0 q:50 := Consts.equal T p q
+
+variables [cT : Consistent T] {L}
+include cT
+
+lemma Tω_consistent' : consistent (theory_limit L T) := Tω_consistent T cT.consis
+
+lemma mem_Tω'_of_Tω_provable {p : formula Lω} (b : Tω ⊢ p): p ∈ Tω⁺ :=
+begin
+  have : Tω⁺ ⊢ p, from weakening' (Tω_consistent' T).ss_maximal b,
+  exact (Tω_consistent' T).mem_maximal_iff.mpr this
+end
+
+@[simp, refl] lemma Consts.equal_refl (c : Consts L) : c ~[T] c := by simp[Consts.equal, (Tω_consistent' T).mem_maximal_iff]
+
+theorem Consts.equal_equivalence : equivalence (Consts.equal T) :=
+⟨λ p, by simp[Consts.equal, (Tω_consistent' T).mem_maximal_iff],
+  λ p q, by { simp[Consts.equal, (Tω_consistent' T).mem_maximal_iff], exact provable.eq_symm },
+  λ p q r, by { simp[Consts.equal, (Tω_consistent' T).mem_maximal_iff], exact provable.eq_trans }⟩
+
+lemma Consts.of_eq (t : term Lω) :
+ t ≃∘ Consts.of t ∈ Tω⁺ :=
+begin
+  have : ∐ (t^1 ≃∘ #0) ⟶ (t ≃∘ Consts.of t) ∈ Tω, by simpa[Consts.fn] using henkin_mem_Tω L T (t^1 ≃ #0),
+  have lmm₁ : Tω ⊢ ∐ (t^1 ≃∘ #0) ⟶ (t ≃∘ Consts.of t), from by_axiom this,
+  have lmm₂ : Tω ⊢ ∐ (t^1 ≃∘ #0), from provable.use t (by simp),
+  have : Tω ⊢ t ≃∘ Consts.of t, from lmm₁ ⨀ lmm₂,
+  exact mem_Tω'_of_Tω_provable T this
+end
+
+lemma Consts.fn_eq {n} (f : (limit L).fn n) (v : finitary (Consts L) n) :
+ (app f (λ i, (v i)) ≃∘ Consts.fn f v) ∈ Tω⁺ :=
+Consts.of_eq _ _
+
+@[reducible, simp, instance]
+def henkin : setoid (Consts L) := ⟨Consts.equal T, Consts.equal_equivalence T⟩
+
+def Henkin : Type u := quotient (henkin T)
+
+namespace Henkin
+variables {T}
+
+@[elab_as_eliminator]
+protected lemma ind_on {C : Henkin T → Prop} (d : Henkin T)
+  (h : ∀ p : Consts L, C ⟦p⟧) : C d :=
+quotient.induction_on' d h
+
+@[elab_as_eliminator, reducible]
+def lift_on {φ} (d : Henkin T) (f : Consts L → φ)
+  (h : ∀ p q : Consts L, p ~[T] q → f p = f q) : φ :=
+quotient.lift_on' d f h
+
+@[simp]
+lemma lift_on_eq {φ} (p : Consts L) (f : Consts L → φ)
+  (h : ∀ p q : Consts L, p ~[T] q → f p = f q) : lift_on ⟦p⟧ f h = f p := rfl
+
+@[elab_as_eliminator, reducible, simp]
+def lift_on₂ {φ} (d₁ d₂ : Henkin T) (f : Consts L → Consts L → φ)
+  (h : ∀ p₁ p₂ q₁ q₂, p₁ ~[T] q₁ → p₂ ~[T] q₂ → f p₁ p₂ = f q₁ q₂) : φ :=
+quotient.lift_on₂' d₁ d₂ f h
+
+@[simp] lemma lift_on₂_eq {φ} (p q : Consts L) (f : Consts L → Consts L → φ)
+  (h : ∀ p₁ p₂ q₁ q₂, p₁ ~[T] q₁ → p₂ ~[T] q₂ → f p₁ p₂ = f q₁ q₂) :
+lift_on₂ ⟦p⟧ ⟦q⟧ f h = f p q := rfl
+
+def lift_on_finitary {φ} {n : ℕ} (v : finitary (Henkin T) n) (f : finitary (Consts L) n → φ)
+  (h : ∀ v₁ v₂ : finitary (Consts L) n, (∀ n, (v₁ n) ~[T] (v₂ n)) → f v₁ = f v₂) : φ :=
+quotient.lift_on_finitary v f h 
+
+@[simp] lemma lift_on_finitary_eq {φ} {n} (v : finitary (Consts L) n) (f : finitary (Consts L) n → φ)
+  (h : ∀ v₁ v₂ : finitary (Consts L) n, (∀ n, (v₁ n) ~[T] (v₂ n)) → f v₁ = f v₂) :
+  lift_on_finitary (λ x, ⟦v x⟧) f h = f v :=
+quotient.lift_on_finitary_eq v f h
+
+@[simp] lemma of_eq_of {p q : Consts L} : (⟦p⟧ : Henkin T) = ⟦q⟧ ↔ p ~[T] q := quotient.eq'
+
+def fn {n} (f : (Lω).fn n) : finitary (Henkin T) n → Henkin T :=
+λ v, lift_on_finitary v (λ v, (⟦Consts.fn f v⟧ : Henkin T)) $ λ v₁ v₂ eqs,
+begin
+  simp[of_eq_of, Consts.equal, (Tω_consistent' T).mem_maximal_iff],
+  show      Tω⁺ ⊢ Consts.fn f v₁ ≃∘ Consts.fn f v₂,
+  have b₁ : Tω⁺ ⊢ app f (λ i, (v₁ i)) ≃∘ Consts.fn f v₁, from (Tω_consistent' T).mem_maximal_iff.mp (Consts.fn_eq T f v₁),
+  have b₂ : Tω⁺ ⊢ app f (λ i, (v₂ i)) ≃∘ Consts.fn f v₂, from (Tω_consistent' T).mem_maximal_iff.mp (Consts.fn_eq T f v₂),
+  have b  : Tω⁺ ⊢ app f (λ i, (v₁ i)) ≃∘ app f (λ i, (v₂ i)),
+  { have : ∀ i, Tω⁺ ⊢ v₁ i ≃∘ v₂ i, from λ i, (Tω_consistent' T).mem_maximal_iff.mp (eqs i),
+    have : Tω⁺ ⊢ ⋀ i, v₁ i ≃∘ v₂ i, refine fopl.provable.conjunction' this,
+    exact function_ext' f (λ i, (v₁ i)) (λ i, (v₂ i)) ⨀ this },
+  exact eq_trans (eq_trans b₁.eq_symm b) b₂
+end
+
+@[simp] lemma fn_app {n} (f : (Lω).fn n) (v : finitary (Consts L) n) :
+  fn f (λ i, ⟦v i⟧) = ⟦Consts.fn f v⟧ :=
+lift_on_finitary_eq _ _ _
+
+def pr {n} (r : (Lω).pr n) : finitary (Henkin T) n → Prop :=
+λ v, lift_on_finitary v (Consts.pr T r) $ λ v₁ v₂ eqs,
+begin
+  simp[of_eq_of, Consts.pr, (Tω_consistent' T).mem_maximal_iff],
+  suffices : Tω⁺ ⊢ app r (λ i, (v₁ i)) ⟷ app r (λ i, (v₂ i)),
+  { split; intros h, { exact (iff_equiv.mp this).1 ⨀ h }, { exact (iff_equiv.mp this).2 ⨀ h } },
+  have : ∀ i, Tω⁺ ⊢ v₁ i ≃∘ v₂ i, from λ i, (Tω_consistent' T).mem_maximal_iff.mp (eqs i),
+  have : Tω⁺ ⊢ ⋀ i, v₁ i ≃∘ v₂ i, refine fopl.provable.conjunction' this,
+  exact predicate_ext'' r (λ i, (v₁ i)) (λ i, (v₂ i)) ⨀ this
+end
+
+@[simp] lemma pr_app {n} (r : (Lω).pr n) (v : finitary (Consts L) n) :
+  pr r (λ i, ⟦v i⟧) ↔ formula.app r (λ i, (v i)) ∈ Tω⁺ :=
+by { have : pr r (λ i, ⟦v i⟧) = Consts.pr T r v, from lift_on_finitary_eq _ _ _, simp[this, Consts.pr] }
+
+variables (T)
+
+def henkin_model : model Lω := ⟨Henkin T, ⟨⟦henkin_constant ⊤⟧⟩, λ n f, fn f, λ n r, pr r⟩
+
+local notation `ℌ` := henkin_model T
+
+
+@[simp] lemma henkin_model_fn {n} (f : (Lω).fn n) (v) : (ℌ).fn f v = fn f v := rfl
+@[simp] lemma henkin_model_pr {n} (r : (Lω).pr n) (v) : (ℌ).pr r v = pr r v := rfl
+
+lemma eq_Consts_of_eq {t u} : Consts.of t ~[T] Consts.of u ↔ Tω⁺ ⊢ t ≃∘ u  :=
+begin
+  simp[Consts.equal, (Tω_consistent' T).mem_maximal_iff],
+  have lmm₁ : Tω⁺ ⊢ t ≃∘ Consts.of t, from by_axiom (Consts.of_eq T _), 
+  have lmm₂ : Tω⁺ ⊢ u ≃∘ Consts.of u, from by_axiom (Consts.of_eq T _), 
+  refine ⟨λ h, eq_trans (eq_trans lmm₁ h) (eq_symm lmm₂), λ h, eq_trans (eq_trans (eq_symm lmm₁) h) lmm₂⟩
+end
+
+lemma term_val_eq_quotient (t : term Lω) (e : ℕ → Consts L) :
+  @term.val _ ℌ (λ n, ⟦e n⟧ : ℕ → |ℌ|) t = ⟦Consts.of (t.rew (λ x, ↑(e x)))⟧ :=
+begin
+  induction t,
+  case var : x { simp[Consts.equal], exact Consts.of_eq T _ },
+  case app : n f v IH
+  { simp,
+    have : (λ i, @term.val _ ℌ (λ n, ⟦e n⟧) (v i)) = (λ i, ⟦Consts.of ((v i).rew (λ x, ↑(e x)))⟧),
+    { funext i, exact IH i },
+    simp[this, Consts.fn],
+    have : Tω⁺ ⊢ app f (λ i, (Consts.of ((v i).rew (λ x, (e x))))) ≃∘ app f (λ i, (v i).rew (λ x, (e x))),
+    { have : ∀ i, Tω⁺ ⊢ Consts.of ((v i).rew (λ x, (e x))) ≃∘ (v i).rew (λ x, (e x)),
+        from λ i, eq_symm (by_axiom (Consts.of_eq T ((v i).rew (λ x, (e x))))),
+      have : Tω⁺ ⊢ ⋀ i, Consts.of ((v i).rew (λ x, (e x))) ≃∘ (v i).rew (λ x, (e x)),
+        from fopl.provable.conjunction' this,
+      exact function_ext' f _ _ ⨀ this },
+    refine (eq_Consts_of_eq _).mpr this }
+end
+
+private lemma ℌ_models_Tω'_fal
+  {p : formula Lω} 
+  (IH : ∀ (s : ℕ → Consts L), p.rew (λ x, ↑(s x)) ∈ Tω⁺ ↔ @formula.val _ ℌ (λ x, ⟦s x⟧) p)
+  (s : ℕ → Consts L) :
+  (∏ p).rew (λ x, ↑(s x)) ∈ Tω⁺ ↔ ℌ ⊧[λ x, ⟦s x⟧] (∏ p) :=
+begin
+  simp, split,
+    { intros h,  intros c,
+      induction c using fopl.henkin.Henkin.ind_on,
+      let s' : ℕ → Consts L := c ⌢ s,
+      have : p.rew (λ x, (s' x)) ∈ Tω⁺,
+      { simp[(Tω_consistent' T).mem_maximal_iff] at h ⊢,
+        have : Tω⁺ ⊢ p.rew (c ⌢ λ x, (s x)),  simpa[formula.nested_rew] using h ⊚ c,
+        simpa using this },
+      simpa[s', app_concat c s] using (IH s').1 this },
+    { intros h,
+      have h : ∀ (c : Consts L), @formula.val _ ℌ (λ x, ⟦(c ⌢ s) x⟧) p, { intros c, simp, exact h ⟦c⟧ },
+      by_contradiction A,
+      let φ := ⁻p.rew ((λ x, (s x))^1),
+      have lmm₁ : Tω⁺ ⊢  p.rew (henkin_constant φ ⌢ (λ x, (s x))),
+        by simpa using by_axiom ((IH _).mpr (h $ henkin_constant φ)),         
+      have : Tω⁺ ⊢ ⁻∏ p.rew ((λ x, (s x))^1), from by_axiom ((Tω_consistent' T).neg_mem_maximal_iff.mpr A),      
+      have : Tω⁺ ⊢ ∐ φ, from (iff_of_equiv (provable.neg_fal_equiv_ex_neg _)).mp this,
+      have lmm₂ : Tω⁺ ⊢ ⁻p.rew (henkin_constant φ ⌢ (λ x, (s x))),
+        by simpa[φ, formula.nested_rew] using by_axiom ((Tω_consistent' T).ss_maximal (henkin_mem_Tω L T φ)) ⨀ this,
+      exact (Tω_consistent' T).maximal_consistent ⟨_, lmm₁, lmm₂⟩ }
+end
+
+theorem ℌ_models_Tω' (p : formula Lω) (s : ℕ → Consts L) :
+  p.rew (λ x, ↑(s x)) ∈ Tω⁺ ↔ ℌ ⊧[λ x, ⟦s x⟧] p :=
+begin
+  induction p generalizing s,
+  case app : n r v
+  { simp[term_val_eq_quotient, (Tω_consistent' T).mem_maximal_iff],
+    suffices :  Tω⁺ ⊢ app r (λ i, (v i).rew (λ x, (s x))) ⟷ app r (λ i, Consts.of ((v i).rew (λ x, (s x)))), from iff_of_equiv this,
+    have : ∀ i, Tω⁺ ⊢ (v i).rew (λ x, (s x)) ≃∘ Consts.of ((v i).rew (λ x, (s x))),
+      from λ i, (by_axiom (Consts.of_eq T ((v i).rew (λ x, (s x))))),
+    have :      Tω⁺ ⊢ ⋀ i, (v i).rew (λ x, (s x)) ≃∘ Consts.of ((v i).rew (λ x, (s x))),
+      from fopl.provable.conjunction' this,
+    exact predicate_ext'' r _ _ ⨀ this },
+  case equal : t u { simp[term_val_eq_quotient, (Tω_consistent' T).mem_maximal_iff], exact iff.symm (eq_Consts_of_eq _) },
+  case imply : p q IH_p IH_q { simp[(Tω_consistent' T).imply_mem_maximal_iff] at*, simp[IH_p s, IH_q s] },
+  case verum { simp[(Tω_consistent' T).mem_maximal_iff] },
+  case neg : p IH { simp[(Tω_consistent' T).neg_mem_maximal_iff], exact iff.not (IH s) },
+  case fal : p IH { exact ℌ_models_Tω'_fal T IH s }
+end
+
+theorem ℌ_models_Tω'_of_sentence {p : formula Lω} (hp : sentence p) :
+  p ∈ Tω⁺ ↔ ℌ ⊧ p :=
+by simpa[hp, eval_sentence_iff] using ℌ_models_Tω' T p default
+
+variables [closed_theory T]
+
+theorem ℌ_models_T : add_left.of_ltr ℌ ⊧ₜₕ T :=
+begin
+  simp[theory_models_iff], intros p mem,
+  have : p ∈ Tω⁺, from (Tω_consistent' T).ss_maximal (T_ss_Tω T mem),  
+  exact (ℌ_models_Tω'_of_sentence T (show sentence p, from closed_theory.cl mem)).mp this
+end 
+
+end Henkin
+
 end henkin
+
+variables [closed_theory T] {L} {T}
+
+theorem exists_model_of_consistent (consis : T.consistent) : ∃ M, M ⊧ₜₕ T :=
+⟨_, @henkin.Henkin.ℌ_models_T _ T ⟨consis⟩ _⟩
+
+theorem completeness {p : formula L} (hp : sentence p) : 
+  T ⊢ p ↔ (∀ M, M ⊧ₜₕ T → M ⊧ p) :=
+⟨λ b M hM, soundness b hM,
+ λ h, by { simp[theory.provable_iff_inconsistent], intros consis,
+  have : closed_theory (T +{⁻p}), from ⟨by { simp[hp], sorry}⟩,
+  have : ∃ M, M ⊧ₜₕ (T +{⁻p}), exactI exists_model_of_consistent consis,
+  rcases this with ⟨M, hM⟩,
+  have : M ⊧ p, from h M (λ p mem, hM p (by simp[mem])),
+  have : ¬M ⊧ p, by simpa[model.models_neg_iff_of_sentence hp] using hM (⁻p) (by simp),
+  contradiction }⟩
 
 end fopl
